Clean/Ironwood.lean
@@ -22,6 +22,8 @@ import Clean.Ironwood.NoteCommit.YComposite
 import Clean.Ironwood.NoteCommit.Main
 import Clean.Ironwood.CommitIvk.Gadget
 import Clean.Ironwood.NoteCommit.MainBundle
+import Clean.Ironwood.CommitIvk.Main
+import Clean.Ironwood.CommitIvk.MainBundle
 import Clean.Ironwood.Utilities.AddChip
 import Clean.Ironwood.Poseidon.Pow5
 import Clean.Ironwood.Poseidon.Rounds
